---
description: Express trigonometric expressions in complex form
topics:
  - complex numbers
  - trigonometry
  - periodic motion
difficulty: medium
status: solved
interested: false
book: Vibrations and Waves
chapter: Superposition of periodic motions
---

## Problem Statement
Express the following in the form $z = Re[Ae^{i(\omega t+\alpha)}]$
(a) $z = \sin \omega t + \cos \omega t$.
(b) $z = \cos(\omega t - \pi/3) - \cos \omega t$.
(c) $z = 2\sin \omega t + 3\cos \omega t$.
(d) $z = \sin \omega t - 2\cos(\omega t - \pi/4) + \cos \omega t$.

## Solution 

(a)

When $z$ is maximal it would be that $Re[Ae^{i(\omega t)}] = Ae^{i\alpha} = A$

That gives us A

$$\begin{align*}
t = 0&: z = 1 \\
\omega t = \frac{\pi}{8}&: z = \sqrt{2} \\
\omega t = \frac{\pi}{4}&: z = 1 \\
\omega t = \frac{3\pi}{8}&: z = 0 \\
\frac{\pi}{2}&: z = -1
\end{align*}$$

So $A = \sqrt{2}$ and $\alpha = -\frac{\pi}{8}$

$$\begin{align*}
Re[\sqrt{2}e^{i(\omega t - \frac{\pi}{8})}] &= \sqrt{2}\cos(\omega t - \frac{\pi}{8}) \\
&= \sqrt{2}\cos\omega t\cos\frac{\pi}{8} + \sin\omega t\sin\frac{\pi}{8} \\
&= \frac{\sqrt{2}}{\sqrt{2}}(\cos\omega t + \sin\omega t) \\
&= \cos\omega t + \sin\omega t
\end{align*}$$

Okay âœ“

(b) $z = \cos(\omega t - \pi/3) - \cos\omega t$

where is it max? $z' = \omega(\sin\omega t - \sin(\omega t - \pi/3))$

$\sin\omega t - \sin(\omega t - \frac{\pi}{3}) = 0$

$$\begin{align*}
\sin\omega t - (\sin\omega t\cos\frac{\pi}{3} + \cos\omega t\sin\frac{\pi}{3}) &= 0 \\
\sin\omega t(1 - \frac{1}{2}) + \cos\omega t\frac{\sqrt{3}}{2} &= 0 \\
\frac{\sin\omega t}{\cos\omega t} &= -\sqrt{3} \text{ Thus the max}
\end{align*}$$

Back to formula

$\tan\omega t = -\sqrt{3}$

$\omega t = -\frac{\pi}{3}$

$\cos(-\frac{2\pi}{3}) - \cos(-\frac{\pi}{3}) = -\frac{1}{2} - \frac{1}{2} = -1$

So $A = 1$ and for min $\omega t + \alpha = -\pi$ so $\alpha = -\pi + \frac{\pi}{3} = -\frac{2\pi}{3}$

$z = Re[e^{i(\omega t + \frac{2\pi}{3})}]$

(c) Ahh wait maybe there's an easier way. The general form is:
$$\begin{align*}
z = Re[Ae^{i(\omega t + \alpha)}] &= A\cos(\omega t + \alpha) \\
&= A(\cos\omega t\cos\alpha - \sin\omega t\sin\alpha)
\end{align*}$$

So $$\begin{bmatrix} A\cos\alpha \\ -A\sin\alpha \end{bmatrix} = \begin{bmatrix} 3 \\ 2 \end{bmatrix}$$ I think we can use the same trick

$\tan\alpha = -\frac{2}{3}$

$\cos\alpha = \frac{3}{\sqrt{13}} \Rightarrow A = \sqrt{13}, \alpha = -0.588$

(d) $$\begin{align*}
z &= \sin\omega t - 2\cos(\omega t - \pi/4) + \cos\omega t \\
&= \sin\omega t - 2(\cos\frac{\pi}{4}\cos\omega t + \sin\frac{\pi}{4}\sin\omega t) + \cos\omega t \\
&= (1 - 2\cos\frac{\pi}{4})\cos\omega t + (1 - 2\sin\frac{\pi}{4})\sin\omega t \\
&= (1 - \sqrt{2})(\cos\omega t + \sin\omega t)
\end{align*}$$

We already solved this, $A = \sqrt{2}, \alpha = -\frac{\pi}{8}$

We get $Re[\sqrt{3} - 2)e^{i(\omega t - \frac{\pi}{8})}] = Re[(2 - \sqrt{2})e^{i(\omega t + \frac{7\pi}{8})}]$