---
description: Find electric field of infinite wire using potential method
topics:
  - electrostatics
  - infinite wire
  - potential
  - field
difficulty: medium
status: solved
interested: false
book: Electricity and Magnetism
chapter: The electric potential
---

## Problem Statement
Consider the electric field E due to an infinite straight wire with uniform linear charge density Î». In Section 1.12 we found E by direct integration of Coulomb's law, and again by using Gauss's law. Find E here by calculating the potential and then taking the derivative.

You will find that the potential (relative to infinity) due to an infinite wire diverges. But you can get around this difficulty by instead finding the potential due to a very long but finite wire of length 2L, at a point lying on its perpendicular bisecting plane. Use a Taylor series to simplify your result, and then take the derivative to find E. Explain why this procedure is valid, even though it cuts off an infinite amount from the potential.

## Solution 

$$
\begin{align*}
\frac{1}{4\pi\epsilon_0} \int \frac{dq}{r} &= \frac{1}{4\pi\epsilon_0} \int \frac{\lambda dx}{\sqrt{x^2+s^2}} \\
&= \frac{\lambda}{4\pi\epsilon_0} \int_{-L}^L \frac{dx}{\sqrt{x^2+s^2}}
\end{align*}
$$

Here we have:
* $\frac{x}{s} = \sinh \alpha$
* $\sqrt{(\frac{x}{s})^2+1} = \cosh \alpha$
* $\frac{dx}{s} = \cosh \alpha d\alpha$

$$
\begin{align*}
&= \frac{\lambda}{4\pi\epsilon_0} \int_{\sinh^{-1}(-\frac{L}{s})}^{\sinh^{-1}(\frac{L}{s})} \frac{1}{\cosh \alpha} \cosh \alpha d\alpha \\
&= \frac{\lambda}{4\pi\epsilon_0}\left[\sinh^{-1}(\frac{L}{s}) - \sinh^{-1}(-\frac{L}{s})\right] \\
&= \frac{\lambda}{2\pi\epsilon_0}\sinh^{-1}\left(\frac{L}{s}\right)
\end{align*}
$$

Develop Taylor series. Around which point?

From symmetry we know gradient points to or away from line.

### wrong turn

Let's try at $s_0=L$ so:

$$\phi(s) = \frac{\lambda}{4\pi\epsilon_0}\left[\sinh^{-1}(1) + \frac{1}{\sqrt{2}}\frac{1}{L}(s-L) + ...\right]$$

$$\frac{d(\sinh^{-1}\frac{L}{s})}{ds}(s_0) = \frac{1}{\sqrt{(\frac{L}{s_0})^2+1}} \cdot \frac{-L}{s_0^2}$$

$$\frac{d^2\sinh^{-1}\frac{L}{s}}{ds^2}(s_0) = \frac{-1}{2\left((\frac{L}{s_0})^2+1\right)^{3/2}} \cdot 2\frac{L}{s_0}\frac{-L}{s_0^2} + \frac{1}{\sqrt{(\frac{L}{s_0})^2+1}}\frac{2L}{s_0^3}$$

The rest of the terms in the Taylor series go as $O(s^n)$:

$$\phi'(s) = \frac{\lambda}{2\pi\epsilon_0} \cdot \frac{1}{\sqrt{s}}\frac{1}{L}$$

### better approach

Okay I think it's a mistake to evaluate at $s_0$ that depends on $L$, so let's just keep it as a parameter for now.

$$\phi'(s) = \frac{\lambda}{2\pi\epsilon_0}\left[\frac{-L}{s_0^2\sqrt{(\frac{L}{s_0})^2+1}} + ...\right]$$

$$-\sqrt{\frac{L^2}{s_0^4(\frac{L^2}{s_0^2}+1)}} = -\sqrt{\frac{1}{s_0^2+\frac{1}{L}}} \xrightarrow{L\to\infty} -\frac{1}{s_0}$$

Let us justify several key steps in our derivation:

1. **Radial Symmetry and the Electric Field**

The potential $\phi$ is generally a function of all spatial coordinates. However, on the perpendicular bisecting plane, the problem exhibits radial symmetry about the wire axis. This means $\phi$ depends only on the radial distance $s$ from the wire.

To show that $\frac{d\phi}{ds} = |\nabla\phi|$, we can use the chain rule. In cylindrical coordinates $(s,\theta,z)$, where $z$ is along the wire:

$$
\begin{align*}
\nabla\phi &= \frac{\partial\phi}{\partial s}\hat{s} + \frac{1}{s}\frac{\partial\phi}{\partial\theta}\hat{\theta} + \frac{\partial\phi}{\partial z}\hat{z} \\
&= \frac{d\phi}{ds}\hat{s}
\end{align*}
$$

The $\theta$ and $z$ terms vanish due to symmetry. Therefore, $|\nabla\phi| = |\frac{d\phi}{ds}|$, and the electric field $\vec{E} = -\nabla\phi$ points radially (inward or outward).

2. **Convergence of the Taylor Series**

While the potential of an infinite wire diverges at infinity, our approach using a finite wire of length $2L$ and then taking $L\to\infty$ is valid for several reasons:

a) The coefficients in our Taylor series, when examined as functions of $L$, converge as $L\to\infty$. This can be seen from the balanced powers of $L$ in numerators and denominators of the derivatives.

b) Electrostatic potentials are defined only up to an additive constant. Different choices of reference point will only affect the constant term in the Taylor series. Since we ultimately take the derivative to find $\vec{E}$, this constant term is irrelevant.

## Author solution
Okay, looked at the solution, I think the approach I used is flawed. Here's what the author did:

$$\phi(s) = \frac{\lambda}{4\pi\epsilon_0}\left[\log(\sqrt{x^2+s^2} + x)\right]^L_{-L}$$

$$= \frac{\lambda}{4\pi\epsilon_0}\log\left(\frac{\sqrt{L^2+s^2} + L}{\sqrt{L^2+s^2} - L}\right)$$

$$= \frac{\lambda}{4\pi\epsilon_0}\log\left(\frac{\sqrt{1+\frac{s^2}{L^2}} + 1}{\sqrt{1+\frac{s^2}{L^2}} - 1}\right)$$

Now, when $L \gg s$ then using the Taylor approx around $x_0 = 0$ of $\sqrt{1+x} = 1 + \frac{1}{2}\frac{1}{1+0}x$

we get $\sqrt{1+\frac{s^2}{L^2}} \approx 1 + \frac{s^2}{2L^2}$

and so $\frac{\sqrt{1+\frac{s^2}{L^2}} + 1}{\sqrt{1+\frac{s^2}{L^2}} - 1} \approx \frac{\frac{s^2}{2L^2} + 2}{\frac{s^2}{2L^2}} = \frac{s^2 + 4L^2}{s^2} = 1 + \frac{4L^2}{s^2}$

Again for $L \gg s$ This is basically $\frac{4L^2}{s^2}$. plugging it back to the log we get

$$\phi(s) = \frac{\lambda}{4\pi\epsilon_0}\log\frac{4L^2}{s^2} = \frac{\lambda}{2\pi\epsilon_0}(\log 2L - \log s)$$

Now even though $\log 2L \xrightarrow{L\to\infty} \infty$ it is constant in $s$ so we discard it and are left with

$$\phi(s) = -\frac{\lambda}{2\pi\epsilon_0}\log(s)$$

and $E(s) = -\frac{\partial\phi}{\partial s} = \frac{\lambda}{2\pi\epsilon_0}\frac{1}{s}$

Why is this answer better? To me it seems more straight forward with assumptions that are better contained. We get rid of the higher order Taylor terms early and with reasonable justification.

Still, perhaps a simpler case can be made just by looking at the limit of the derivative I found before

$$\phi'(s) = -\frac{\lambda}{2\pi\epsilon_0}\frac{1}{\sqrt{s^2+\frac{1}{L}}}$$