---
description: Calculate potential at different points from charged rod
topics:
  - electrostatics
  - potential
  - integration
difficulty: medium
status: solved
interested: false
book: Electricity and Magnetism
chapter: The electric potential
---

## Problem Statement
A thin rod extends along the z axis from z = -d to z = d. The rod carries a charge uniformly distributed along its length with linear charge density Î». By integrating over this charge distribution, calculate the potential at a point $P_1$ on the z axis with coordinates (0, 0, 2d). By another integration find the potential at a general point $P_2$ on the x axis and locate this point to make the potential equal to the potential at $P_1$.

## Solution 

A thin rod extends along the z axis from $z = -d$ to $z = d$. The rod carries a charge uniformly distributed along its length with linear charge density $\lambda$.

Calculate potential at $P_1 = (0,0,2d)$

Calculate potential at $P_2 = (x,0,0)$

Find $x$ such that $V(P_1) = V(P_2)$

For $P_1$:
$$\begin{align*}
V(P_1) &= \frac{1}{4\pi\epsilon_0} \int \frac{dq}{r} = \frac{1}{4\pi\epsilon_0} \int \frac{\lambda}{2d-l} dl \\
&= \frac{\lambda}{4\pi\epsilon_0} [-\log(2d-l)]_{-d}^d \\
&= \frac{\lambda}{4\pi\epsilon_0}(-\log d + \log 3d) \\
&= \frac{\lambda}{4\pi\epsilon_0}\log 3
\end{align*}$$

For $P_2$:
$$\begin{align*}
V(P_2) &= \frac{\lambda}{4\pi\epsilon_0} \int_{-d}^d \frac{1}{\sqrt{l^2+x^2}} dl = \frac{\lambda}{4\pi\epsilon_0} \int_{-d}^d \frac{1}{x\sqrt{(\frac{l}{x})^2+1}} dl \\
&= \frac{\lambda}{4\pi\epsilon_0} \int_{-d/x}^{d/x} \frac{1}{\sqrt{1+y^2}} dy \\
&= \frac{\lambda}{4\pi\epsilon_0}[\sinh^{-1}y]_{-d/x}^{d/x} \\
&= \frac{\lambda}{4\pi\epsilon_0}[\log(\frac{d}{x} + \sqrt{(\frac{d}{x})^2+1}) - \log(\frac{-d}{x} + \sqrt{(\frac{d}{x})^2+1})] \\
&= \frac{\lambda}{4\pi\epsilon_0}\log(\frac{\frac{d}{x} + \sqrt{(\frac{d}{x})^2+1}}{-\frac{d}{x} + \sqrt{(\frac{d}{x})^2+1}})
\end{align*}$$

So this $\log$ should be equal to 3:

$$\begin{align*}
\frac{d}{x} + \sqrt{(\frac{d}{x})^2+1} &= 3\sqrt{(\frac{d}{x})^2+1} - 3\frac{d}{x} \\
\sqrt{(\frac{d}{x})^2+1} - 2\frac{d}{x} &= 0 \\
(\frac{d}{x})^2+1 - 4(\frac{d}{x})^2 &= 0 \\
\frac{d}{x} &= \sqrt{\frac{1}{3}}
\end{align*}$$

Therefore: $x = \sqrt{3}d$

Let's verify:
$$\frac{\frac{1}{\sqrt{3}} + \sqrt{\frac{1}{3}+1}}{-\frac{1}{\sqrt{3}} + \sqrt{\frac{1}{3}+1}} = \frac{3}{\sqrt{3}}/\frac{1}{\sqrt{3}} = 3$$